<?xml version="1.0"?>
<rdf:RDF xmlns="https://w3id.org/kpxl/rel/terms/ScientificRelationsOntology#"
     xml:base="https://w3id.org/kpxl/rel/terms/ScientificRelationsOntology"
     xmlns:owl="http://www.w3.org/2002/07/owl#"
     xmlns:rdf="http://www.w3.org/1999/02/22-rdf-syntax-ns#"
     xmlns:xml="http://www.w3.org/XML/1998/namespace"
     xmlns:xsd="http://www.w3.org/2001/XMLSchema#"
     xmlns:rdfs="http://www.w3.org/2000/01/rdf-schema#"
     xmlns:skos="http://www.w3.org/2004/02/skos/core#"
     xmlns:vann="http://purl.org/vocab/vann/"
     xmlns:terms="http://purl.org/dc/terms/">
    <owl:Ontology rdf:about="https://w3id.org/kpxl/rel/terms/ScientificRelationsOntology">
        <terms:creator rdf:resource="https://orcid.org/0000-0002-1267-0234"/>
        <terms:description>The Scientific Relations Ontology defines some general relations between classes.</terms:description>
        <terms:license rdf:resource="https://creativecommons.org/publicdomain/zero/1.0/"/>
        <terms:title>Scientific Relations Ontology</terms:title>
        <vann:preferredNamespacePrefix>rel</vann:preferredNamespacePrefix>
        <vann:preferredNamespaceUri>https://w3id.org/kpxl/rel/terms/</vann:preferredNamespaceUri>
        <rdfs:isDefinedBy rdf:resource="https://w3id.org/kpxl/rel/latest/tendsToAffect"/>
    </owl:Ontology>
    


    <!-- 
    ///////////////////////////////////////////////////////////////////////////////////////
    //
    // Annotation properties
    //
    ///////////////////////////////////////////////////////////////////////////////////////
     -->


    


    <!-- http://purl.org/dc/terms/creator -->


    <owl:AnnotationProperty rdf:about="http://purl.org/dc/terms/creator"/>
    


    <!-- http://purl.org/dc/terms/description -->


    <owl:AnnotationProperty rdf:about="http://purl.org/dc/terms/description"/>
    


    <!-- http://purl.org/dc/terms/license -->


    <owl:AnnotationProperty rdf:about="http://purl.org/dc/terms/license"/>
    


    <!-- http://purl.org/dc/terms/title -->


    <owl:AnnotationProperty rdf:about="http://purl.org/dc/terms/title"/>
    


    <!-- http://purl.org/vocab/vann/preferredNamespacePrefix -->


    <owl:AnnotationProperty rdf:about="http://purl.org/vocab/vann/preferredNamespacePrefix"/>
    


    <!-- http://purl.org/vocab/vann/preferredNamespaceUri -->


    <owl:AnnotationProperty rdf:about="http://purl.org/vocab/vann/preferredNamespaceUri"/>
    


    <!-- http://www.w3.org/2004/02/skos/core#definition -->


    <owl:AnnotationProperty rdf:about="http://www.w3.org/2004/02/skos/core#definition"/>
    


    <!-- 
    ///////////////////////////////////////////////////////////////////////////////////////
    //
    // Object Properties
    //
    ///////////////////////////////////////////////////////////////////////////////////////
     -->


    


    <!-- https://w3id.org/kpxl/rel/terms/tendsToAffect -->


    <owl:ObjectProperty rdf:about="https://w3id.org/kpxl/rel/terms/tendsToAffect">
        <rdfs:domain rdf:resource="http://www.w3.org/2002/07/owl#Class"/>
        <rdfs:range rdf:resource="http://www.w3.org/2002/07/owl#Class"/>
        <rdfs:isDefinedBy rdf:resource="https://w3id.org/kpxl/rel/latest/tendsToAffect"/>
        <rdfs:label xml:lang="en">has instances that tend to affect instances of</rdfs:label>
        <rdfs:seeAlso rdf:resource="https://w3id.org/linkflows/superpattern/terms/affects"/>
        <skos:definition xml:lang="en">the instances of the subject tend to positively or negatively affect the intensity or frequency of activity instances of the object</skos:definition>
    </owl:ObjectProperty>
    


    <!-- https://w3id.org/kpxl/rel/terms/tendsToBeCausedBy -->


    <owl:ObjectProperty rdf:about="https://w3id.org/kpxl/rel/terms/tendsToBeCausedBy">
        <rdfs:domain rdf:resource="http://www.w3.org/2002/07/owl#Class"/>
        <rdfs:range rdf:resource="http://www.w3.org/2002/07/owl#Class"/>
        <rdfs:isDefinedBy rdf:resource="https://w3id.org/kpxl/rel/latest/tendsToBeCausedBy"/>
        <rdfs:label xml:lang="en">has instances that tend to be caused by instances of</rdfs:label>
        <rdfs:seeAlso rdf:resource="https://w3id.org/linkflows/superpattern/terms/causes"/>
        <skos:definition xml:lang="en">the instances of the subject tend to cause the existence of instances of the object</skos:definition>
    </owl:ObjectProperty>
    


    <!-- https://w3id.org/kpxl/rel/terms/tendsToBeFollowedBy -->


    <owl:ObjectProperty rdf:about="https://w3id.org/kpxl/rel/terms/tendsToBeFollowedBy">
        <rdfs:domain rdf:resource="http://www.w3.org/2002/07/owl#Class"/>
        <rdfs:range rdf:resource="http://www.w3.org/2002/07/owl#Class"/>
        <rdfs:isDefinedBy rdf:resource="https://w3id.org/kpxl/rel/latest/tendsToBeFollowedBy"/>
        <rdfs:label xml:lang="en">has instances that tend to be followed by instances of</rdfs:label>
        <rdfs:seeAlso rdf:resource="https://w3id.org/linkflows/superpattern/terms/isFollowedBy"/>
        <skos:definition xml:lang="en">the instances of the subject tend to come into existence before instances of the object</skos:definition>
    </owl:ObjectProperty>
    


    <!-- https://w3id.org/kpxl/rel/terms/tendsToBeIncludedIn -->


    <owl:ObjectProperty rdf:about="https://w3id.org/kpxl/rel/terms/tendsToBeIncludedIn">
        <rdfs:domain rdf:resource="http://www.w3.org/2002/07/owl#Class"/>
        <rdfs:range rdf:resource="http://www.w3.org/2002/07/owl#Class"/>
        <rdfs:isDefinedBy rdf:resource="https://w3id.org/kpxl/rel/latest/tendsToBeIncludedIn"/>
        <rdfs:label xml:lang="en">has instances that tend to be included in instances of</rdfs:label>
        <rdfs:seeAlso rdf:resource="https://w3id.org/linkflows/superpattern/terms/isIncludedIn"/>
        <skos:definition xml:lang="en">the instances of the subject tend to be spatiotemporally included in instances of the object</skos:definition>
    </owl:ObjectProperty>
    


    <!-- https://w3id.org/kpxl/rel/terms/tendsToBeNecessaryAndSufficientFor -->


    <owl:ObjectProperty rdf:about="https://w3id.org/kpxl/rel/terms/tendsToBeNecessaryAndSufficientFor">
        <rdfs:domain rdf:resource="http://www.w3.org/2002/07/owl#Class"/>
        <rdfs:range rdf:resource="http://www.w3.org/2002/07/owl#Class"/>
        <rdfs:isDefinedBy rdf:resource="https://w3id.org/kpxl/rel/latest/tendsToBeNecessaryAndSufficientFor"/>
        <rdfs:label xml:lang="en">has instances that tend to be necessary and sufficient for instances of</rdfs:label>
        <rdfs:seeAlso rdf:resource="https://w3id.org/linkflows/superpattern/terms/isNecessaryAndSufficientFor"/>
        <skos:definition xml:lang="en">the instances of the subject tend to cause the existence of instances of the object, which would not exist if the subject instances did not exist</skos:definition>
    </owl:ObjectProperty>
    


    <!-- https://w3id.org/kpxl/rel/terms/tendsToCause -->


    <owl:ObjectProperty rdf:about="https://w3id.org/kpxl/rel/terms/tendsToCause">
        <rdfs:domain rdf:resource="http://www.w3.org/2002/07/owl#Class"/>
        <rdfs:range rdf:resource="http://www.w3.org/2002/07/owl#Class"/>
        <rdfs:isDefinedBy rdf:resource="https://w3id.org/kpxl/rel/latest/tendsToCause"/>
        <rdfs:label xml:lang="en">has instances that tend to cause instances of</rdfs:label>
        <rdfs:seeAlso rdf:resource="https://w3id.org/linkflows/superpattern/terms/causes"/>
        <skos:definition xml:lang="en">the instances of the subject tend to cause the existence of instances of the object</skos:definition>
    </owl:ObjectProperty>
    


    <!-- https://w3id.org/kpxl/rel/terms/tendsToContributeTo -->


    <owl:ObjectProperty rdf:about="https://w3id.org/kpxl/rel/terms/tendsToContributeTo">
        <rdfs:domain rdf:resource="http://www.w3.org/2002/07/owl#Class"/>
        <rdfs:range rdf:resource="http://www.w3.org/2002/07/owl#Class"/>
        <rdfs:isDefinedBy rdf:resource="https://w3id.org/kpxl/rel/latest/tendsToContributeTo"/>
        <rdfs:label xml:lang="en">has instances that tend to contribute to instances of</rdfs:label>
        <rdfs:seeAlso rdf:resource="https://w3id.org/linkflows/superpattern/terms/contributesTo"/>
        <skos:definition xml:lang="en">the instances of the subject tend to positively affect the intensity or frequency of activity instances of the object</skos:definition>
    </owl:ObjectProperty>
    


    <!-- https://w3id.org/kpxl/rel/terms/tendsToCooccurWith -->


    <owl:ObjectProperty rdf:about="https://w3id.org/kpxl/rel/terms/tendsToCooccurWith">
        <rdfs:domain rdf:resource="http://www.w3.org/2002/07/owl#Class"/>
        <rdfs:range rdf:resource="http://www.w3.org/2002/07/owl#Class"/>
        <rdfs:isDefinedBy rdf:resource="https://w3id.org/kpxl/rel/latest/tendsToCooccurWith"/>
        <rdfs:label xml:lang="en">has instances that tend to co-occur with instances of</rdfs:label>
        <rdfs:seeAlso rdf:resource="https://w3id.org/linkflows/superpattern/terms/coOccursWith"/>
        <skos:definition xml:lang="en">the instances of the subject tend to be close to instances of the object in terms of space and time</skos:definition>
    </owl:ObjectProperty>
    


    <!-- https://w3id.org/kpxl/rel/terms/tendsToDecrease -->


    <owl:ObjectProperty rdf:about="https://w3id.org/kpxl/rel/terms/tendsToDecrease">
        <rdfs:domain rdf:resource="http://www.w3.org/2002/07/owl#Class"/>
        <rdfs:range rdf:resource="http://www.w3.org/2002/07/owl#Class"/>
        <rdfs:isDefinedBy rdf:resource="https://w3id.org/kpxl/rel/latest/tendsToDecrease"/>
        <rdfs:label xml:lang="en">has instances that tend to decrease instances of</rdfs:label>
        <rdfs:seeAlso rdf:resource="https://w3id.org/linkflows/superpattern/terms/decreases"/>
        <skos:definition xml:lang="en">the instances of the subject tend to cause the value of instances of the object to decrease</skos:definition>
    </owl:ObjectProperty>
    


    <!-- https://w3id.org/kpxl/rel/terms/tendsToEnable -->


    <owl:ObjectProperty rdf:about="https://w3id.org/kpxl/rel/terms/tendsToEnable">
        <rdfs:domain rdf:resource="http://www.w3.org/2002/07/owl#Class"/>
        <rdfs:range rdf:resource="http://www.w3.org/2002/07/owl#Class"/>
        <rdfs:isDefinedBy rdf:resource="https://w3id.org/kpxl/rel/latest/tendsToEnable"/>
        <rdfs:label xml:lang="en">has instances that tend to enable instances of</rdfs:label>
        <rdfs:seeAlso rdf:resource="https://w3id.org/linkflows/superpattern/terms/enables"/>
        <skos:definition xml:lang="en">the instances of the subject tend to cause activity instances of the object to happen</skos:definition>
    </owl:ObjectProperty>
    


    <!-- https://w3id.org/kpxl/rel/terms/tendsToFollow -->


    <owl:ObjectProperty rdf:about="https://w3id.org/kpxl/rel/terms/tendsToFollow">
        <rdfs:domain rdf:resource="http://www.w3.org/2002/07/owl#Class"/>
        <rdfs:range rdf:resource="http://www.w3.org/2002/07/owl#Class"/>
        <rdfs:isDefinedBy rdf:resource="https://w3id.org/kpxl/rel/latest/tendsToFollow"/>
        <rdfs:label xml:lang="en">has instances that tend to follow instances of</rdfs:label>
        <rdfs:seeAlso rdf:resource="https://w3id.org/linkflows/superpattern/terms/follows"/>
        <skos:definition xml:lang="en">the instances of the subject tend to come into existence after instances of the object</skos:definition>
    </owl:ObjectProperty>
    


    <!-- https://w3id.org/kpxl/rel/terms/tendsToHaveDifferentValueFrom -->


    <owl:ObjectProperty rdf:about="https://w3id.org/kpxl/rel/terms/tendsToHaveDifferentValueFrom">
        <rdfs:domain rdf:resource="http://www.w3.org/2002/07/owl#Class"/>
        <rdfs:range rdf:resource="http://www.w3.org/2002/07/owl#Class"/>
        <rdfs:isDefinedBy rdf:resource="https://w3id.org/kpxl/rel/latest/tendsToHaveDifferentValueFrom"/>
        <rdfs:label xml:lang="en">has instances that tend to have a different value from instances of</rdfs:label>
        <rdfs:seeAlso rdf:resource="https://w3id.org/linkflows/superpattern/terms/hasDifferentValueFrom"/>
        <skos:definition xml:lang="en">the quantifiable instances of the subject tend to have a value that is different from quantifiable instances of the object</skos:definition>
    </owl:ObjectProperty>
    


    <!-- https://w3id.org/kpxl/rel/terms/tendsToHaveLargerValueThan -->


    <owl:ObjectProperty rdf:about="https://w3id.org/kpxl/rel/terms/tendsToHaveLargerValueThan">
        <rdfs:domain rdf:resource="http://www.w3.org/2002/07/owl#Class"/>
        <rdfs:range rdf:resource="http://www.w3.org/2002/07/owl#Class"/>
        <rdfs:isDefinedBy rdf:resource="https://w3id.org/kpxl/rel/latest/tendsToHaveLargerValueThan"/>
        <rdfs:label xml:lang="en">has instances that tend to have a larger value than instances of</rdfs:label>
        <rdfs:seeAlso rdf:resource="https://w3id.org/linkflows/superpattern/terms/hasLargerValueThan"/>
        <skos:definition xml:lang="en">the quantifiable instances of the subject tend to have a larger value than quantifiable instances of the object</skos:definition>
    </owl:ObjectProperty>
    


    <!-- https://w3id.org/kpxl/rel/terms/tendsToHaveSameValueAs -->


    <owl:ObjectProperty rdf:about="https://w3id.org/kpxl/rel/terms/tendsToHaveSameValueAs">
        <rdfs:domain rdf:resource="http://www.w3.org/2002/07/owl#Class"/>
        <rdfs:range rdf:resource="http://www.w3.org/2002/07/owl#Class"/>
        <rdfs:isDefinedBy rdf:resource="https://w3id.org/kpxl/rel/latest/tendsToHaveSameValueAs"/>
        <rdfs:label xml:lang="en">has instances that tend to have the same value as instances of</rdfs:label>
        <rdfs:seeAlso rdf:resource="https://w3id.org/linkflows/superpattern/terms/hasSameValueAs"/>
        <skos:definition xml:lang="en">the quantifiable instances of the subject tend to have the same value as quantifiable instances of the object</skos:definition>
    </owl:ObjectProperty>
    


    <!-- https://w3id.org/kpxl/rel/terms/tendsToHaveSimilarValueAs -->


    <owl:ObjectProperty rdf:about="https://w3id.org/kpxl/rel/terms/tendsToHaveSimilarValueAs">
        <rdfs:domain rdf:resource="http://www.w3.org/2002/07/owl#Class"/>
        <rdfs:range rdf:resource="http://www.w3.org/2002/07/owl#Class"/>
        <rdfs:isDefinedBy rdf:resource="https://w3id.org/kpxl/rel/latest/tendsToHaveSimilarValueAs"/>
        <rdfs:label xml:lang="en">has instances that tend to have a similar value as instances of</rdfs:label>
        <rdfs:seeAlso rdf:resource="https://w3id.org/linkflows/superpattern/terms/hasSimilarValueAs"/>
        <skos:definition xml:lang="en">the quantifiable instances of the subject tend to have a similar value as quantifiable instances of the object</skos:definition>
    </owl:ObjectProperty>
    


    <!-- https://w3id.org/kpxl/rel/terms/tendsToHaveSmallerValueThan -->


    <owl:ObjectProperty rdf:about="https://w3id.org/kpxl/rel/terms/tendsToHaveSmallerValueThan">
        <rdfs:domain rdf:resource="http://www.w3.org/2002/07/owl#Class"/>
        <rdfs:range rdf:resource="http://www.w3.org/2002/07/owl#Class"/>
        <rdfs:isDefinedBy rdf:resource="https://w3id.org/kpxl/rel/latest/tendsToHaveSmallerValueThan"/>
        <rdfs:label xml:lang="en">has instances that tend to have a smaller value than instances of</rdfs:label>
        <rdfs:seeAlso rdf:resource="https://w3id.org/linkflows/superpattern/terms/hasSmallerValueThan"/>
        <skos:definition xml:lang="en">the quantifiable instances of the subject tend to have a smaller value than quantifiable instances of the object</skos:definition>
    </owl:ObjectProperty>
    


    <!-- https://w3id.org/kpxl/rel/terms/tendsToInclude -->


    <owl:ObjectProperty rdf:about="https://w3id.org/kpxl/rel/terms/tendsToInclude">
        <rdfs:domain rdf:resource="http://www.w3.org/2002/07/owl#Class"/>
        <rdfs:range rdf:resource="http://www.w3.org/2002/07/owl#Class"/>
        <rdfs:isDefinedBy rdf:resource="https://w3id.org/kpxl/rel/latest/tendsToInclude"/>
        <rdfs:label xml:lang="en">has instances that tend to include instances of</rdfs:label>
        <rdfs:seeAlso rdf:resource="https://w3id.org/linkflows/superpattern/terms/includes"/>
        <skos:definition xml:lang="en">the instances of the subject tend to spatiotemporally include instances of the object</skos:definition>
    </owl:ObjectProperty>
    


    <!-- https://w3id.org/kpxl/rel/terms/tendsToIncrease -->


    <owl:ObjectProperty rdf:about="https://w3id.org/kpxl/rel/terms/tendsToIncrease">
        <rdfs:domain rdf:resource="http://www.w3.org/2002/07/owl#Class"/>
        <rdfs:range rdf:resource="http://www.w3.org/2002/07/owl#Class"/>
        <rdfs:isDefinedBy rdf:resource="https://w3id.org/kpxl/rel/latest/tendsToIncrease"/>
        <rdfs:label xml:lang="en">has instances that tend to increase instances of</rdfs:label>
        <rdfs:seeAlso rdf:resource="https://w3id.org/linkflows/superpattern/terms/increases"/>
        <skos:definition xml:lang="en">the instances of the subject tend to cause the value of instances of the object to increase</skos:definition>
    </owl:ObjectProperty>
    


    <!-- https://w3id.org/kpxl/rel/terms/tendsToInhibit -->


    <owl:ObjectProperty rdf:about="https://w3id.org/kpxl/rel/terms/tendsToInhibit">
        <rdfs:domain rdf:resource="http://www.w3.org/2002/07/owl#Class"/>
        <rdfs:range rdf:resource="http://www.w3.org/2002/07/owl#Class"/>
        <rdfs:isDefinedBy rdf:resource="https://w3id.org/kpxl/rel/latest/tendsToInhibit"/>
        <rdfs:label xml:lang="en">has instances that tend to inhibit instances of</rdfs:label>
        <rdfs:seeAlso rdf:resource="https://w3id.org/linkflows/superpattern/terms/inhibits"/>
        <skos:definition xml:lang="en">the instances of the subject tend to negatively affect the intensity or frequency of the activity instances of the object</skos:definition>
    </owl:ObjectProperty>
    


    <!-- https://w3id.org/kpxl/rel/terms/tendsToPrevent -->


    <owl:ObjectProperty rdf:about="https://w3id.org/kpxl/rel/terms/tendsToPrevent">
        <rdfs:domain rdf:resource="http://www.w3.org/2002/07/owl#Class"/>
        <rdfs:range rdf:resource="http://www.w3.org/2002/07/owl#Class"/>
        <rdfs:isDefinedBy rdf:resource="https://w3id.org/kpxl/rel/latest/tendsToPrevent"/>
        <rdfs:label xml:lang="en">has instances that tend to prevent instances of</rdfs:label>
        <rdfs:seeAlso rdf:resource="https://w3id.org/linkflows/superpattern/terms/prevents"/>
        <skos:definition xml:lang="en">the instances of the subject tend to cause the activity instances of the object not to happen</skos:definition>
    </owl:ObjectProperty>
    


    <!-- https://w3id.org/kpxl/rel/terms/tendsToRequire -->


    <owl:ObjectProperty rdf:about="https://w3id.org/kpxl/rel/terms/tendsToRequire">
        <rdfs:domain rdf:resource="http://www.w3.org/2002/07/owl#Class"/>
        <rdfs:range rdf:resource="http://www.w3.org/2002/07/owl#Class"/>
        <rdfs:isDefinedBy rdf:resource="https://w3id.org/kpxl/rel/latest/tendsToRequire"/>
        <rdfs:label xml:lang="en">has instances that tend to require instances of</rdfs:label>
        <rdfs:seeAlso rdf:resource="https://w3id.org/linkflows/superpattern/terms/requires"/>
        <skos:definition xml:lang="en">the instances of the subject tend not to have existed if instances of the object did not exist</skos:definition>
    </owl:ObjectProperty>
    


    <!-- 
    ///////////////////////////////////////////////////////////////////////////////////////
    //
    // Classes
    //
    ///////////////////////////////////////////////////////////////////////////////////////
     -->


    


    <!-- http://www.w3.org/2002/07/owl#Class -->


    <owl:Class rdf:about="http://www.w3.org/2002/07/owl#Class"/>
</rdf:RDF>



<!-- Generated by the OWL API (version 5.1.18) https://github.com/owlcs/owlapi/ -->


